examples/List_Reversal.thy
@@ -2,6 +2,9 @@ theory List_Reversal
   imports "ITree_UTP.ITree_UTP"
 begin lit_vars
 
+syntax
+  "_kleisli_comp" :: "logic \<Rightarrow> logic \<Rightarrow> logic" (infixr ";" 54)
+
 def_consts MAX_SIL_STEPS = 100
 
 zstore state =
@@ -9,9 +12,19 @@ zstore state =
   i :: nat
 
 procedure reverse "xs :: int list" over state =
-"ys := [] \<Zcomp> i := 0 \<Zcomp> while i < length xs inv ys = rev (take i xs) do ys := xs!i # ys \<Zcomp> i := i + 1 od"
+"ys := [] ; i := 0 ; 
+ while i < length xs inv ys = rev (take i xs) 
+ do 
+    ys := xs!i # ys; 
+    i := i + 1 
+ od"
+
+procedure reverse' "xs :: int list" over state =
+"ys := [];
+ for j in [0..<length xs] do ys := xs!j # ys od"
 
 execute "reverse [1,2,3,4]"
+execute "reverse' [1,2,3,4]"
 
 lemma reverse_correct: "H{True} reverse xs {ys = rev xs}"
   unfolding reverse_def
